src/dvspec/dafny/att_spec_proofs/ind_inv.dfy
@@ -5,7 +5,8 @@ include "../specification/consensus.dfy"
 include "../specification/network.dfy"
 include "../specification/dvn.dfy"
 include "../att_spec_proofs/inv.dfy"
-include "../att_spec_proofs/fnc_inv.dfy"
+include "../att_spec_proofs/fnc_invs_1_26.dfy"
+include "../att_spec_proofs/fnc_invs_27.dfy"
 include "../att_spec_proofs/dvn_next_invs_1_7.dfy"
 include "../att_spec_proofs/dvn_next_invs_8_18.dfy"
 include "../att_spec_proofs/dvn_next_invs_19_26.dfy"
@@ -21,6 +22,7 @@ module Att_Ind_Inv_With_Empty_Initial_Attestation_Slashing_DB
     import opened Att_Inv_With_Empty_Initial_Attestation_Slashing_DB
     import opened Helper_Sets_Lemmas
     import opened Fnc_Invs_1_26   
+    import opened Fnc_Invs_27   
     import opened DVN_Next_Invs_1_7
     import opened DVN_Next_Invs_8_18
     import opened DVN_Next_Invs_19_26
